finish the implement of ex7

ass1/Ex7.dfy
@@ -1,27 +1,42 @@
-predicate Occourance(a :array<int>, key: int, count: int, last:int)
-requires 0 <= last < a.Length
-decreases  a, count, last
+function method doOccourance(a: array<int>, key: int, last:int):int
+    requires 0 <= last < a.Length 
+    decreases last
+    reads a
 {
-    if(last > 0) then 
-        if (a[last]== key)
-        then 
-            Occourance(a, key,count -1 , last -1)
+    if (last == 0) then 
+        if( a[last] == key) then 
+            1
+        else
+            0
+    else 
+        if( a[last] == key) then 
+            doOccourance(a,key,last -1) + 1
         else 
-            Occourance(a, key, count, last -1)
-    else
-        // last == 0 
-        a[0] == key ==> count == 1 && a[0] != key ==> count == 0
+            doOccourance(a,key,last -1)
+        
 }
 
 
+function method Occourance(a: array<int>, key: int):int
+    reads a 
+{
+    if(a.Length == 0) then 
+        0
+    else 
+        doOccourance(a,key, a.Length -1)
+}
 
 method Just1(a: array<int>, key: int) returns (b: bool)
+    ensures b ==(1  == Occourance(a,key))
 {
     var count:= 0;
     var i := 0;
 
     while (i < a.Length)
-    
+        invariant 0<= i <= a.Length
+        // if statement in the loop inv 
+        invariant 0 < i <= a.Length ==> count == doOccourance(a,key, i-1)
+        invariant i == 0            ==> count == 0
         decreases a.Length - i 
     {
         if(a[i]== key){
